lib/seplog/Loops.v
@@ -1,7 +1,6 @@
 Set Implicit Arguments.
-From SLF Require Import Fun LabType Sum ListCommon.
-From SLF Require Import LibSepReference LibWP LibSepSimpl Struct.
-From SLF Require Import LibSepTLCbuffer.
+From LGTM.lib.theory Require Import LibFunExt LibLabType LibSummation LibListExt LibSepTLCbuffer.
+From LGTM.lib.seplog Require Import LibSepReference LibWP LibSepSimpl Struct.
 From mathcomp Require Import ssreflect ssrfun zify.
 Hint Rewrite conseq_cons' : rew_listx.
 
@@ -1765,7 +1764,7 @@ Proof.
     move: Hd. erewrite -> NoDup_nth in Hnodup. apply Hnodup; math. }
   erewrite hbig_fset_eq with (fs:=`[0, N]). 1: xsimpl*. 2: move=> * /=; by rewrite hbig_fset_label_single'.
   erewrite hbig_fset_eq. 1: xsimpl*. 
-  move=> d Hnotin /=. rewrite filter_indom indom_interval /Sum.mem /= in Hnotin. do 2 f_equal. now apply Hpre.
+  move=> d Hnotin /=. rewrite filter_indom indom_interval /LibSummation.mem /= in Hnotin. do 2 f_equal. now apply Hpre.
 Qed.
 
 (* TODO it might be easier to change some_eq to be on some type A, and use the toval trick again 
@@ -1874,7 +1873,7 @@ Proof.
   (* TODO the following part is very bad; need improvement *)
   move=> hv. rewrite hstar_fset_hexists. xsimpl*=> vl.
   rewrite hstar_fset_pure_hstar. xsimpl*=> Hvl. setoid_rewrite indom_interval in Hvl.
-  pose (vl' := fun i : int => If In i idx then vl (ListCommon.index i idx) else (nth (abs i) arr1 def)).
+  pose (vl' := fun i : int => If In i idx then vl (LibListExt.index i idx) else (nth (abs i) arr1 def)).
   eapply himpl_trans. 2: apply (PostH hv vl'). 
   assert (forall i0 : int, 0 <= i0 < M -> some_eq (vl' i0) (nth (abs i0) (arr2 hv) def)) as Htmp.
   { intros i0 Hi0. rewrite /vl'. case_if.
@@ -1893,8 +1892,482 @@ Proof.
   2: move=> d Hd /=; rewrite indom_interval in Hd; specialize (Hidx d Hd); rewrite hbig_fset_label_single' Hl1 /vl' ?index_nodup //; try math.
   2: assert (In idx[d] idx) by (apply nth_In; math); case_if; eqsolve.
   erewrite hbig_fset_eq. 1: xsimpl*. 
-  move=> d Hnotin /=. rewrite filter_indom indom_interval /Sum.mem /= in Hnotin. f_equal. 
+  move=> d Hnotin /=. rewrite filter_indom indom_interval /LibSummation.mem /= in Hnotin. f_equal. 
   rewrite Hl1 /vl'; try math. case_if; eqsolve.
+Qed.
+
+
+Lemma xfor_lemma_gen_array_fun_aux `{ID : Inhab D}
+  Inv 
+  (R R' : Dom -> hhprop)
+  s fsi1 vr (arrl : loc) (f : int -> int) (g : _ -> _ -> int) (idx : list int)
+  (N M:int) (C1 : Dom -> trm) (C : trm)
+  (i j : int)
+  Pre Post: 
+  length idx = N :> int ->
+  NoDup idx ->
+  (forall (l : int), 
+    (0 <= l < N) -> 0 <= idx[l] < M) ->
+  (forall (l : int), 
+    (0 <= l < N) ->
+    {{ Inv l \* 
+        (\*_(d <- ⟨(j,0)%Z, fsi1 l⟩) R d) \* 
+        (arrl + 1 + abs (idx[l]))%nat ~⟨(i,0)%Z, s⟩~> f (idx[l]) }}
+      [{
+        {i| _  in single s tt  => subst vr l C};
+        {j| ld in fsi1 l       => C1 ld}
+      }]
+    {{ v, 
+        Inv (l + 1) \* 
+        (\*_(d <- ⟨(j,0)%Z, fsi1 l⟩) R' d) \* 
+        (arrl + 1 + abs (idx[l]))%nat ~⟨(i,0)%Z, s⟩~> g v (idx[l]) }}) ->
+  (forall j : int, hlocal (Inv j) ⟨(i,0%Z), single s tt⟩) ->
+  (forall i : Dom, hlocal (R i) ⟨(j,0%Z), (single i tt)⟩) ->
+  (forall i : Dom, hlocal (R' i) ⟨(j,0%Z), (single i tt)⟩) ->
+  (forall (hv hv' : D -> val) m,
+    0 <= m < N ->
+    (forall i, indom (fsi1 m) i -> hv[`j](i) = hv'[`j](i)) ->
+    g hv (idx[m]) = g hv' (idx[m])) ->
+  (forall (hv : D -> val) m,
+    0 <= m < M -> ~ In m idx -> f m = g hv m) ->
+  (i <> j)%Z ->
+  0 <= N <= M ->
+  (forall t : val, subst "for" t C = C) -> 
+  (forall t : val, subst "cnt" t C = C) ->
+  (forall t : val, subst "cond" t C = C) ->
+  var_eq vr "cnt" = false ->
+  var_eq vr "for" = false ->
+  var_eq vr "cond" = false ->
+  (Pre ==> 
+    Inv 0 \* 
+    (\*_(d <- Union `[0,N] fsi1) R d) \*
+    harray_fun_int f arrl M (Lab (i,0) s)) ->
+  (forall hv, 
+    Inv N \* 
+    (\*_(d <- Union `[0,N] fsi1) R' d) \* 
+    harray_fun_int (g hv) arrl M (Lab (i,0) s) ==>
+    Post hv) -> 
+  {{ Pre }}
+    [{
+      {i| _  in single s tt => For 0 N (trm_fun vr C)};
+      {j| ld in Union `[0,N] fsi1 => C1 ld}
+    }]
+  {{ v, Post v }}. 
+Proof.
+  move=>lenidx nodup_idx idx_bounded IH *.
+  eapply xfor_lemma_gen_array with (R := R) (R' := R') (arr1 := LibList.map val_int (lof f M)) (arr2 := fun hv => LibList.map val_int (lof (g hv) M)) (arrl:=arrl) (def:=val_int 0) (some_eq:=eq); try eassumption.
+  1: constructor; hnf; congruence. 
+  { move=> ?; rewrite map_conversion map_length length_lof; math. }
+  { rewrite map_conversion map_length length_lof; math. }
+  { move=> l P; rewrite map_conversion map_nth nth_lof' //; try math; auto.
+    apply/ntriple_conseq; [apply (IH l P) | |move=> v; rewrite map_conversion map_nth nth_lof'//; try math; auto]; xsimpl*. }
+  all: try (move=> *; rewrite ?map_conversion ?map_nth ?nth_lof' //; f_equal; try math; auto).
+  xsimpl=>HH. eapply himpl_trans. 2: eauto. xsimpl*.
+  rewrite /harray_fun_int/harray_int map_conversion.
+  rewrite -(lof_indices) !(lof_indices') in HH |- *.
+  eapply eq_ind_r with (y:=map _ _); [ xsimpl* | ].
+  apply map_ext_in=> a /In_lof_id Hin /=. rewrite HH ?(nth_map_lt 0) ?nth_lof' ?length_lof' //; try math.
+Qed.
+
+
+Lemma xfor_lemma_gen_array_fun `{ID : Inhab D}
+  Inv 
+  (R R' : Dom -> hhprop)
+  s fsi1 vr (arrl : loc) (f : int -> int) (g : _ -> _ -> int) (idx : list int)
+  (N M : Z) (C1 : Dom -> trm) (C C' : trm)
+  (i j : Z)
+  Pre Post: 
+  length idx = N :> int ->
+  NoDup idx ->
+  (forall (l : int), 
+    (0 <= l < N) -> 0 <= idx[l] < M) ->
+  (forall (l : int), 
+    (0 <= l < N) ->
+    {{ Inv l \* 
+        (\*_(d <- ⟨(j,0)%Z, fsi1 l⟩) R d) \* 
+        (arrl + 1 + abs (idx[l]))%nat ~⟨(i,0)%Z, s⟩~> f (idx[l]) }}
+      [{
+        {i| _  in single s tt  => subst vr l C};
+        {j| ld in fsi1 l       => C1 ld}
+      }]
+    {{ v, 
+        Inv (l + 1) \* 
+        (\*_(d <- ⟨(j,0)%Z, fsi1 l⟩) R' d) \* 
+        (arrl + 1 + abs (idx[l]))%nat ~⟨(i,0)%Z, s⟩~> g v (idx[l]) }}) ->
+  (forall j : int, hlocal (Inv j) ⟨(i,0%Z), single s tt⟩) ->
+  (forall i : Dom, hlocal (R i) ⟨(j,0%Z), (single i tt)⟩) ->
+  (forall i : Dom, hlocal (R' i) ⟨(j,0%Z), (single i tt)⟩) ->
+  (forall (hv hv' : D -> val) m,
+    0 <= m < N ->
+    (forall i, indom (fsi1 m) i -> hv[`j](i) = hv'[`j](i)) ->
+    g hv (idx[m]) = g hv' (idx[m])) ->
+  (forall (hv : D -> val) m,
+    0 <= m < M -> ~ In m idx -> f m = g hv m) ->
+  (i <> j)%Z ->
+  0 <= N <= M ->
+  (forall t : val, subst "for" t C = C) -> 
+  (forall t : val, subst "cnt" t C = C) ->
+  (forall t : val, subst "cond" t C = C) ->
+  var_eq vr "cnt" = false ->
+  var_eq vr "for" = false ->
+  var_eq vr "cond" = false ->
+  (Pre ==> 
+    Inv 0 \* 
+    (\*_(d <- Union `[0,N] fsi1) R d) \*
+    harray_fun_int f arrl M (Lab (i,0) s)) ->
+  (forall hv, 
+    Inv N \* 
+    (\*_(d <- Union `[0,N] fsi1) R' d) \* 
+    harray_fun_int (g hv) arrl M (Lab (i,0) s) ==>
+    wp ⟨(i,0),single s tt⟩ (fun=> C') (fun hr' => Post (lab_fun_upd hr' hv (i,0)))) -> 
+  {{ Pre }}
+    [{
+      {i| _  in single s tt => trm_seq (For 0 N (trm_fun vr C)) C'};
+      {j| ld in Union `[0,N] fsi1 => C1 ld}
+    }]
+  {{ v, Post v }}.
+Proof.
+  intros.
+  xfocus (j,0); rewrite ?eqbxx.
+  have E: (lab_eqb (i, 0) (j,0) = false).
+  { by apply/bool_ext; split=> //; rewrite lab_eqbE=> -[]. }
+  rewrite E/= -xnwp1_lemma /= wp_equiv.
+  apply/htriple_conseq; [|eauto|]; first last.
+  { move=> ?. apply/wp_seq. }
+  rewrite (xnwp1_lemma (FH (single s tt) (fun=> For 0 N <{ fun_ {vr} => {C} }>)) ((i,0))).
+  rewrite -wp_equiv.
+  apply/(@xunfocus_lemma _ (fun hr => WP [ _ in ⟨(i, 0), single s tt⟩  => C' ]
+  { hr'0, Post ((hr \u_ ⟨(j, 0), Union (interval 0 N) fsi1⟩) hr'0) }))=> /=; autos*.
+  { by rewrite E. }
+  move=> ??; fequals; apply/fun_ext_1=> ?. fequals.
+  extens=> -[]??; rewrite /uni; case: classicT=> //.
+  xfocus (i,0); rewrite ?eqbxx lab_eqb_sym E /=.
+  apply/xunfocus_lemma; autos*=> /=.
+  { by rewrite lab_eqb_sym E. }
+  { move=> ??. remember ((_ \u_ _) _); reflexivity. }
+  simpl.
+  apply/xfor_lemma_gen_array_fun_aux; try eassumption; eauto.
+  move=> hv. apply: himpl_trans; [|apply/wp_hv].
+  move: (H17 hv); rewrite wp_equiv=> ?.
+  xapp=> hv'. rewrite -/(lab_fun_upd _ _ _).
+  xsimpl (lab_fun_upd hv' hv (i, 0))=> ?.
+  apply: applys_eq_init; fequals; apply/fun_ext_1=> /=.
+  case=> l x.
+  rewrite /uni ?indom_label_eq; case: classicT.
+  { by case=> <- /=; rewrite lab_eqb_sym E. }
+  case: classicT=> //.
+  case=> <- /=; rewrite eqbxx //.
+Qed.
+
+Lemma xfor_lemma_gen_array_fun_aux2 `{ID : Inhab D}
+  Inv 
+  (R1 R1' R2 R2' : Dom -> hhprop)
+  s fsi1 fsi2 vr (arrl : loc) (f : int -> int) (g : _ -> _ -> int) idx
+  (N M: Z) (C1 C2 : Dom -> trm) (C : trm)
+  (i j k : Z)
+  Pre Post: 
+  length idx = N :> int ->
+  NoDup idx ->
+  (forall (l : int), 
+    (0 <= l < N) -> 0 <= idx[l] < M) ->
+  (forall (l : int), 
+    (0 <= l < N) ->
+    {{ Inv l \* 
+        (\*_(d <- ⟨(j,0)%Z, fsi1 l⟩) R1 d) \* 
+        (\*_(d <- ⟨(k,0)%Z, fsi2 l⟩) R2 d) \* 
+        (arrl + 1 + abs (idx[l]))%nat ~⟨(i,0)%Z, s⟩~> f (idx[l]) }}
+      [{
+        {i| _  in single s tt  => subst vr l C};
+        {j| ld in fsi1 l       => C1 ld};
+        {k| ld in fsi2 l       => C2 ld}
+      }]
+    {{ v, 
+        Inv (l + 1) \* 
+        (\*_(d <- ⟨(j,0)%Z, fsi1 l⟩) R1' d) \* 
+        (\*_(d <- ⟨(k,0)%Z, fsi2 l⟩) R2' d) \* 
+        (arrl + 1 + abs (idx[l]))%nat ~⟨(i,0)%Z, s⟩~> g v (idx[l]) }}) ->
+  (forall j : int, hlocal (Inv j) ⟨(i,0%Z), single s tt⟩) ->
+  (forall i : Dom, hlocal (R1 i) ⟨(j,0%Z), (single i tt)⟩) ->
+  (forall i : Dom, hlocal (R1' i) ⟨(j,0%Z), (single i tt)⟩) ->
+  (forall i : Dom, hlocal (R2 i) ⟨(k,0%Z), (single i tt)⟩) ->
+  (forall i : Dom, hlocal (R2' i) ⟨(k,0%Z), (single i tt)⟩) ->
+  (forall (hv hv' : D -> val) m,
+    0 <= m < N ->
+    (forall i, indom (fsi1 m) i -> hv[`j](i) = hv'[`j](i)) ->
+    (forall i, indom (fsi2 m) i -> hv[`k](i) = hv'[`k](i)) ->
+    g hv (idx[m]) = g hv' (idx[m])) ->
+  (forall (hv : D -> val) m,
+    0 <= m < M -> ~ In m idx -> f m = g hv m) ->
+  (i <> j)%Z ->
+  (j <> k)%Z ->
+  (k <> i)%Z ->
+  0 <= N <= M ->
+  (forall t : val, subst "for" t C = C) -> 
+  (forall t : val, subst "cnt" t C = C) ->
+  (forall t : val, subst "cond" t C = C) ->
+  var_eq vr "cnt" = false ->
+  var_eq vr "for" = false ->
+  var_eq vr "cond" = false ->
+  (Pre ==> 
+    Inv 0 \* 
+    (\*_(d <- Union `[0,N] fsi1) R1 d) \*
+    (\*_(d <- Union `[0,N] fsi2) R2 d) \*
+    harray_fun_int f arrl M (Lab (i,0) s)) ->
+  (forall hv, 
+    Inv N \* 
+    (\*_(d <- Union `[0,N] fsi1) R1' d) \*
+    (\*_(d <- Union `[0,N] fsi2) R2' d) \* 
+    harray_fun_int (g hv) arrl M (Lab (i,0) s) ==>
+     Post hv) -> 
+  {{ Pre }}
+    [{
+      {i| _  in single s tt => (For 0 N (trm_fun vr C))};
+      {j| ld in Union `[0,N] fsi1 => C1 ld};
+      {k| ld in Union `[0,N] fsi2 => C2 ld}
+    }]
+  {{ v, Post v }}.
+Proof.
+  move=>??? IH *.
+  eapply xfor_lemma_gen2_array with (R1 := R1) (R1' := R1') (R2 := R2) (R2' := R2') (arr1 := lof f M) (arr2 := fun hv => lof (g hv) M) (arrl:=arrl); try eassumption.
+  { move=> ?; rewrite length_lof; math. }
+  { apply length_lof; math. }
+  { move=> l P; rewrite nth_lof' //; try math; auto.
+    apply/ntriple_conseq; [ | |move=> v; rewrite nth_lof' //; try math; auto]; try exact:himpl_refl.
+    rewrite -/(ntriple _ _ _).  auto. }
+  all: move=> *; rewrite ?nth_lof' //; autos*.
+Qed.
+
+Lemma xfor_lemma_gen_array_fun2 `{ID : Inhab D}
+  Inv 
+  (R1 R1' R2 R2' : Dom -> hhprop)
+  s fsi1 fsi2 vr (arrl : loc) (f : int -> int) (g : _ -> _ -> int) idx
+  (N M: Z) (C1 C2 : Dom -> trm) (C C' : trm)
+  (i j k : Z)
+  Pre Post: 
+  length idx = N :> int ->
+  NoDup idx ->
+  (forall (l : int), 
+    (0 <= l < N) -> 0 <= idx[l] < M) ->
+  (forall (l : int), 
+    (0 <= l < N) ->
+    {{ Inv l \* 
+        (\*_(d <- ⟨(j,0)%Z, fsi1 l⟩) R1 d) \* 
+        (\*_(d <- ⟨(k,0)%Z, fsi2 l⟩) R2 d) \* 
+        (arrl + 1 + abs (idx[l]))%nat ~⟨(i,0)%Z, s⟩~> f (idx[l]) }}
+      [{
+        {i| _  in single s tt  => subst vr l C};
+        {j| ld in fsi1 l       => C1 ld};
+        {k| ld in fsi2 l       => C2 ld}
+      }]
+    {{ v, 
+        Inv (l + 1) \* 
+        (\*_(d <- ⟨(j,0)%Z, fsi1 l⟩) R1' d) \* 
+        (\*_(d <- ⟨(k,0)%Z, fsi2 l⟩) R2' d) \* 
+        (arrl + 1 + abs (idx[l]))%nat ~⟨(i,0)%Z, s⟩~> g v (idx[l]) }}) ->
+  (forall j : int, hlocal (Inv j) ⟨(i,0%Z), single s tt⟩) ->
+  (forall i : Dom, hlocal (R1 i) ⟨(j,0%Z), (single i tt)⟩) ->
+  (forall i : Dom, hlocal (R1' i) ⟨(j,0%Z), (single i tt)⟩) ->
+  (forall i : Dom, hlocal (R2 i) ⟨(k,0%Z), (single i tt)⟩) ->
+  (forall i : Dom, hlocal (R2' i) ⟨(k,0%Z), (single i tt)⟩) ->
+  (forall (hv hv' : D -> val) m,
+    0 <= m < N ->
+    (forall i, indom (fsi1 m) i -> hv[`j](i) = hv'[`j](i)) ->
+    (forall i, indom (fsi2 m) i -> hv[`k](i) = hv'[`k](i)) ->
+    g hv (idx[m]) = g hv' (idx[m])) ->
+  (forall (hv : D -> val) m,
+    0 <= m < M -> ~ In m idx -> f m = g hv m) ->
+  (i <> j)%Z ->
+  (j <> k)%Z ->
+  (k <> i)%Z ->
+  0 <= N <= M ->
+  (forall t : val, subst "for" t C = C) -> 
+  (forall t : val, subst "cnt" t C = C) ->
+  (forall t : val, subst "cond" t C = C) ->
+  var_eq vr "cnt" = false ->
+  var_eq vr "for" = false ->
+  var_eq vr "cond" = false ->
+  (Pre ==> 
+    Inv 0 \* 
+    (\*_(d <- Union `[0,N] fsi1) R1 d) \*
+    (\*_(d <- Union `[0,N] fsi2) R2 d) \*
+    harray_fun_int f arrl M (Lab (i,0) s)) ->
+  (forall hv, 
+    Inv N \* 
+    (\*_(d <- Union `[0,N] fsi1) R1' d) \*
+    (\*_(d <- Union `[0,N] fsi2) R2' d) \* 
+    harray_fun_int (g hv) arrl M (Lab (i,0) s) ==>
+    wp ⟨(i,0),single s tt⟩ (fun=> C') (fun hr' => Post (lab_fun_upd hr' hv (i,0)))) -> 
+  {{ Pre }}
+    [{
+      {i| _  in single s tt => trm_seq (For 0 N (trm_fun vr C)) C'};
+      {j| ld in Union `[0,N] fsi1 => C1 ld};
+      {k| ld in Union `[0,N] fsi2 => C2 ld}
+    }]
+  {{ v, Post v }}.
+Proof.
+  move=> ?????????????????????? PostH.
+  eapply ntriple_sequ2_gen with (Q' := fun hv=> Inv N \*
+    (\*_(d <- \U_(i <- `[0, N]) fsi1 i) R1' d) \*
+    (\*_(d <- \U_(i <- `[0, N]) fsi2 i) R2' d) \*
+    harray_fun_int (g hv) arrl M (Lab (i,0) s)); autos*=> /=.
+  { apply/xfor_lemma_gen_array_fun_aux2; try eassumption; xsimpl*. }
+  { move=> v; rewrite -wp_equiv; apply: himpl_trans_r.
+    apply/wp_hv; apply: wp_conseq Hwp=> hr ? Qh.
+    setoid_rewrite wp_equiv in PostH; xapp=> hr.
+    xsimpl (lab_fun_upd hr v (i, 0))=> ?; apply:applys_eq_init; f_equal; extens=> -[??].
+    rewrite /uni; case: classicT.
+    { rewrite union_empty_r indom_union_eq ?indom_label_eq.
+      case: ssrbool.ifP=> //. 
+      rewrite /is_true bool_eq_true_eq lab_eqbE /==>->[][][]; eqsolve. } 
+    rewrite indom_label_eq indom_single_eq. 
+    by case: classicT=> // -[]<-<-/= /[! eqbxx]. }
+  rewrite Bool.orb_false_r.
+  case E: (lab_eqb _ _); move: E=> /=.
+  { move<-. rewrite lab_eqbE. eqsolve. }
+  rewrite lab_eqbE. eqsolve.
+Qed.
+
+Lemma xfor_lemma_gen_array_fun_normal `{ID : Inhab D}
+  Inv 
+  (R R' : Dom -> hhprop)
+  s fsi1 vr (arrl : loc) (f : int -> int) (g : _ -> _ -> int)
+  (N: Z) (C1 : Dom -> trm) (C C' : trm)
+  (i j : Z)
+  Pre Post: 
+  (forall (l : int), 
+    (0 <= l < N) ->
+    {{ Inv l \* 
+        (\*_(d <- ⟨(j,0)%Z, fsi1 l⟩) R d) \* 
+        (arrl + 1 + abs l)%nat ~⟨(i,0)%Z, s⟩~> f l }}
+      [{
+        {i| _  in single s tt  => subst vr l C};
+        {j| ld in fsi1 l       => C1 ld}
+      }]
+    {{ v, 
+        Inv (l + 1) \* 
+        (\*_(d <- ⟨(j,0)%Z, fsi1 l⟩) R' d) \* 
+        (arrl + 1 + abs l)%nat ~⟨(i,0)%Z, s⟩~> g v l }}) ->
+  (forall j : int, hlocal (Inv j) ⟨(i,0%Z), single s tt⟩) ->
+  (forall i : Dom, hlocal (R i) ⟨(j,0%Z), (single i tt)⟩) ->
+  (forall i : Dom, hlocal (R' i) ⟨(j,0%Z), (single i tt)⟩) ->
+  (forall (hv hv' : D -> val) m,
+    0 <= m < N ->
+    (forall i, indom (fsi1 m) i -> hv[`j](i) = hv'[`j](i)) ->
+    g hv m = g hv' m) ->
+  (i <> j)%Z ->
+  0 <= N ->
+  (forall t : val, subst "for" t C = C) -> 
+  (forall t : val, subst "cnt" t C = C) ->
+  (forall t : val, subst "cond" t C = C) ->
+  var_eq vr "cnt" = false ->
+  var_eq vr "for" = false ->
+  var_eq vr "cond" = false ->
+  (Pre ==> 
+    Inv 0 \* 
+    (\*_(d <- Union `[0,N] fsi1) R d) \*
+    harray_fun_int f arrl N (Lab (i,0) s)) ->
+  (forall hv, 
+    Inv N \* 
+    (\*_(d <- Union `[0,N] fsi1) R' d) \* 
+    harray_fun_int (g hv) arrl N (Lab (i,0) s) ==>
+    wp ⟨(i,0),single s tt⟩ (fun=> C') (fun hr' => Post (lab_fun_upd hr' hv (i,0)))) -> 
+  {{ Pre }}
+    [{
+      {i| _  in single s tt => trm_seq (For 0 N (trm_fun vr C)) C'};
+      {j| ld in Union `[0,N] fsi1 => C1 ld}
+    }]
+  {{ v, Post v }}.
+Proof.
+  intros.
+  have El : List.length (lof (@id int) N) = abs N :> nat.
+  { match goal with |- ?a = _ => enough (a = N :> int) by math end. apply length_lof; math. }
+  eapply xfor_lemma_gen_array_fun with (idx:=lof (@id int) N) (f:=f) (g:=g) (R:=R) (R':=R'); 
+    try eassumption; try math; eauto.
+  { apply NoDup_nth with (d:=0). intros. rewrite -> ! El in *.
+    replace i0 with (abs i0)%nat in * by math.
+    replace j0 with (abs j0)%nat in * by math. rewrite -> ! nth_lof in *; math. }
+  { intros. rewrite nth_lof; math. }
+  { intros. rewrite nth_lof; try math. auto. }
+  { intros. rewrite nth_lof; try math. auto. }
+  { intros hv m HH HH2. false HH2. replace m with ((lof id N)[m]) by (rewrite nth_lof; math).
+    apply nth_In. math. }
+Qed.
+
+Lemma xfor_lemma_gen_array_fun_normal2 `{ID : Inhab D}
+  Inv 
+  (R1 R1' R2 R2' : Dom -> hhprop)
+  s fsi1 fsi2 vr (arrl : loc) (f : int -> int) (g : _ -> _ -> int)
+  (N: Z) (C1 C2 : Dom -> trm) (C C' : trm)
+  (i j k : Z)
+  Pre Post: 
+  (forall (l : int), 
+    (0 <= l < N) ->
+    {{ Inv l \* 
+        (\*_(d <- ⟨(j,0)%Z, fsi1 l⟩) R1 d) \* 
+        (\*_(d <- ⟨(k,0)%Z, fsi2 l⟩) R2 d) \* 
+        (arrl + 1 + abs l)%nat ~⟨(i,0)%Z, s⟩~> f l }}
+      [{
+        {i| _  in single s tt  => subst vr l C};
+        {j| ld in fsi1 l       => C1 ld};
+        {k| ld in fsi2 l       => C2 ld}
+      }]
+    {{ v, 
+        Inv (l + 1) \* 
+        (\*_(d <- ⟨(j,0)%Z, fsi1 l⟩) R1' d) \* 
+        (\*_(d <- ⟨(k,0)%Z, fsi2 l⟩) R2' d) \* 
+        (arrl + 1 + abs l)%nat ~⟨(i,0)%Z, s⟩~> g v l }}) ->
+  (forall j : int, hlocal (Inv j) ⟨(i,0%Z), single s tt⟩) ->
+  (forall i : Dom, hlocal (R1 i) ⟨(j,0%Z), (single i tt)⟩) ->
+  (forall i : Dom, hlocal (R1' i) ⟨(j,0%Z), (single i tt)⟩) ->
+  (forall i : Dom, hlocal (R2 i) ⟨(k,0%Z), (single i tt)⟩) ->
+  (forall i : Dom, hlocal (R2' i) ⟨(k,0%Z), (single i tt)⟩) ->
+  (forall (hv hv' : D -> val) m,
+    0 <= m < N ->
+    (forall i, indom (fsi1 m) i -> hv[`j](i) = hv'[`j](i)) ->
+    (forall i, indom (fsi2 m) i -> hv[`k](i) = hv'[`k](i)) ->
+    g hv m = g hv' m) ->
+  (i <> j)%Z ->
+  (j <> k)%Z ->
+  (k <> i)%Z ->
+  0 <= N ->
+  (forall t : val, subst "for" t C = C) -> 
+  (forall t : val, subst "cnt" t C = C) ->
+  (forall t : val, subst "cond" t C = C) ->
+  var_eq vr "cnt" = false ->
+  var_eq vr "for" = false ->
+  var_eq vr "cond" = false ->
+  (Pre ==> 
+    Inv 0 \* 
+    (\*_(d <- Union `[0,N] fsi1) R1 d) \*
+    (\*_(d <- Union `[0,N] fsi2) R2 d) \*
+    harray_fun_int f arrl N (Lab (i,0) s)) ->
+  (forall hv, 
+    Inv N \* 
+    (\*_(d <- Union `[0,N] fsi1) R1' d) \* 
+    (\*_(d <- Union `[0,N] fsi2) R2' d) \* 
+    harray_fun_int (g hv) arrl N (Lab (i,0) s) ==>
+    wp ⟨(i,0),single s tt⟩ (fun=> C') (fun hr' => Post (lab_fun_upd hr' hv (i,0)))) -> 
+  {{ Pre }}
+    [{
+      {i| _  in single s tt => trm_seq (For 0 N (trm_fun vr C)) C'};
+      {j| ld in Union `[0,N] fsi1 => C1 ld};
+      {k| ld in Union `[0,N] fsi2 => C2 ld}
+    }]
+  {{ v, Post v }}.
+Proof.
+  intros.
+  have El : List.length (lof (@id int) N) = abs N :> nat.
+  { match goal with |- ?a = _ => enough (a = N :> int) by math end. apply length_lof; math. }
+  eapply xfor_lemma_gen_array_fun2 with (idx:=lof (@id int) N) (f:=f) (g:=g) (R1:=R1) (R2:=R2) (R1':=R1') (R2':=R2'); 
+    try eassumption; try math; eauto.
+  { apply NoDup_nth with (d:=0). intros. rewrite -> ! El in *.
+    replace i0 with (abs i0)%nat in * by math.
+    replace j0 with (abs j0)%nat in * by math. rewrite -> ! nth_lof in *; math. }
+  { intros. rewrite nth_lof; math. }
+  { intros. rewrite nth_lof; try math. auto. }
+  { intros. rewrite nth_lof; try math. auto. }
+  { intros hv m HH HH2. false HH2. replace m with ((lof id N)[m]) by (rewrite nth_lof; math).
+    apply nth_In. math. }
 Qed.
 
 End WithLoops.
@@ -2045,3 +2518,111 @@ Tactic Notation "xset_R_core" constr(dom) ident(R) constr(i) :=
 
 Tactic Notation "xset_R" constr(dom) ident(Inv) ident(R) constr(i) := 
   xset_R_core dom R i; xset_clean R R Inv.
+
+Tactic Notation "xfor_sum_cong_solve2" constr(op) :=
+  let hvE1 := fresh "hvE1" in
+  let hvE2 := fresh "hvE2" in
+  let someindom := fresh "someindom" in
+  intros ???? hvE1 hvE2;  (try case_if=> //; [ ]);  
+  rewrite ?/op; indomE;
+  match goal with 
+  | |- Sum ?a _ = Sum ?a _ => apply fold_fset_eq; intros ?; indomE; intros someindom; extens; intros 
+  | _ => idtac
+  end; try (rewrite hvE1 1?hvE2;
+  [eauto|autorewrite with indomE; try math; 
+    (first [ apply someindom | idtac ])| autorewrite with indomE; try math; 
+    (first [ apply someindom | idtac ])]; simpl; try lia).
+
+Tactic Notation "xfor_arrayset" constr(Inv) constr(R) constr(R') constr(op) constr(f) constr(s) :=
+  eapply (@xfor_lemma_gen_array_fun_normal _ _ Inv R R' _ _ _ s f op);
+  [ intros ??; rewrite ?/Inv ?/R ?/R';
+    xnsimpl
+  | 
+  |
+  |
+  | xfor_sum_cong_solve op
+  |
+  |
+  |
+  |
+  |
+  |
+  |
+  |
+  | rewrite ?/Inv ?/R; rewrite -> ?hbig_fset_hstar; xsimpl
+  | intros ?; rewrite ?/Inv ?/R' ?/op; rewrite -> ?hbig_fset_hstar; xsimpl
+  ]=> //; try (solve [ rewrite ?/Inv ?/R ?/R' /=; xlocal ]); autos*; try math.
+
+Tactic Notation "xfor_arrayset" constr(Inv) constr(R) constr(R') constr(op) constr(f) constr(s) constr(idx) :=
+  eapply (@xfor_lemma_gen_array_fun _ _ Inv R R' _ _ _ s f op idx);
+  [ try math
+  |
+  |
+  | intros ??; rewrite ?/Inv ?/R ?/R';
+    xnsimpl
+  |
+  |
+  |
+  | xfor_sum_cong_solve op
+  |
+  | 
+  |
+  |
+  |
+  |
+  |
+  |
+  |
+  | rewrite ?/Inv ?/R; rewrite -> ?hbig_fset_hstar; xsimpl
+  | intros ?; rewrite ?/Inv ?/R' ?/op; rewrite -> ?hbig_fset_hstar; xsimpl
+  ]=> //; try (solve [ rewrite ?/Inv ?/R ?/R' /=; xlocal ]); autos*; try math.
+
+Tactic Notation "xfor_arrayset" constr(Inv) constr(R1) constr(R1') constr(R2) constr(R2') constr(op) constr(f) constr(s) :=
+  eapply (@xfor_lemma_gen_array_fun_normal2 _ _ Inv R1 R1' R2 R2' _ _ _ _ s f op);
+  [ intros ??; rewrite ?/Inv ?/R1 ?/R1' ?/R2 ?/R2'; xnsimpl
+  |
+  |
+  |
+  |
+  |
+  | xfor_sum_cong_solve2 op
+  |
+  |
+  |
+  |
+  |
+  |
+  |
+  |
+  |
+  |
+  | rewrite ?/Inv ?/R1 /R2; rewrite -> ?hbig_fset_hstar; xsimpl
+  | intros ?; rewrite ?/Inv ?/R1 /R2 ?/op; rewrite -> ?hbig_fset_hstar; xsimpl
+  ]=> //; try (solve [ rewrite ?/Inv ?/R1 ?/R1' ?/R2 ?/R2' /=; xlocal ]); autos*; try math.
+
+Tactic Notation "xfor_arrayset" constr(Inv) constr(R1) constr(R1') constr(R2) constr(R2') constr(op) constr(f) constr(s) constr(idx) :=
+  eapply (@xfor_lemma_gen_array_fun2 _ _ Inv R1 R1' R2 R2' _ _ _ _ s f op idx);
+  [ try math
+  | 
+  | 
+  | intros ??; rewrite ?/Inv ?/R1 ?/R1' ?/R2 ?/R2'; xnsimpl
+  |
+  |
+  |
+  |
+  |
+  | xfor_sum_cong_solve2 op
+  |
+  |
+  |
+  |
+  | 
+  |
+  |
+  |
+  |
+  |
+  |
+  |rewrite ?/Inv ?/R1 ?/R2; rewrite -> ?hbig_fset_hstar; xsimpl
+  | intros ?; rewrite ?/Inv ?/R1' ?/R2' ?/op; rewrite -> ?hbig_fset_hstar; xsimpl
+  ]=> //; try (solve [ rewrite ?/Inv ?/R1 ?/R1' ?/R2 ?/R2' /=; xlocal ]); autos*; try math.
